update typechecker

Coq/Coq35.v
@@ -7,3 +7,101 @@ Require Import Strings.String.
 Add LoadPath "C:\Users\ycy12\Documents\Workspace\LEARNING-STUFF\Coq".
 Load Coq32.
 
+Import STLC.
+
+Fixpoint eqb_ty (T1 T2:ty) : bool :=
+  match T1,T2 with
+  | Bool, Bool =>
+      true
+  | Arrow T11 T12, Arrow T21 T22 =>
+      andb (eqb_ty T11 T21) (eqb_ty T12 T22)
+  | _,_ =>
+      false
+  end.
+
+Lemma eqb_ty_refl : forall T1, eqb_ty T1 T1 = true.
+Proof.
+  intros. induction T1;simpl;auto.
+  rewrite IHT1_1, IHT1_2. auto.
+Qed.
+
+Lemma eqb_ty_eq: forall T1 T2, eqb_ty T1 T2 = true -> T1 = T2.
+Proof.
+  intros T1. induction T1;intros;simpl in *;destruct T2;auto.
+  1 - 2: inversion H.
+  rewrite andb_true_iff in H;destruct H. apply (IHT1_1 T2_1) in H.
+  apply (IHT1_2 T2_2) in H0. subst;auto.
+Qed.
+
+Module STLCChecker.
+  Import STLC.
+
+  Notation " x <- e1 <| e2" := (match e1 with
+                              | Some x => e2
+                              | None => None
+                              end)
+         (right associativity, at level 60).
+
+Notation " 'return' e "
+  := (Some e) (at level 70).
+Notation " 'fail' "
+  := None.
+
+Fixpoint type_check (Gamma : context) (t : tm) : option ty :=
+  match t with
+  | var x =>
+      match Gamma x with
+      | Some T => return T
+      | None => fail
+      end
+  | abs x T11 t12 =>
+      T12 <- type_check (update Gamma x T11) t12 <|
+      return (Arrow T11 T12)
+  | app t1 t2 =>
+      T1 <- type_check Gamma t1 <|
+      T2 <- type_check Gamma t2 <|
+      (match T1 with
+      | Arrow T11 T12 =>
+          if eqb_ty T11 T2 then return T12 else fail
+      | _ => fail
+      end)
+  | tru =>
+      return Bool
+  | fls =>
+      return Bool
+  | test guard t1 t2 =>
+      Tguard <- type_check Gamma guard <|
+      T1 <- type_check Gamma t1 <|
+      T2 <- type_check Gamma t2 <|
+      match Tguard with
+      | Bool =>
+          if eqb_ty T1 T2 then return T1 else fail
+      | _ => fail
+      end
+  end.
+
+Theorem type_checking_sound : ÅÕGamma t T,
+  type_check Gamma t = Some T Å® has_type Gamma t T.
+Proof with eauto.
+  intros Gamma t. generalize dependent Gamma. induction t;intros;simpl in *...
+
+  destruct (Gamma s) eqn: Hn.  inversion H. subst. eauto.
+  inversion H.
+Abort.
+
+Theorem type_checking_complete : ÅÕGamma t T,
+  has_type Gamma t T Å® type_check Gamma t = Some T.
+Proof with auto.
+  intros;induction H;simpl in *.
+
+  destruct (Gamma x0) eqn:H0; assumption.
+  rewrite IHhas_type...
+
+  rewrite IHhas_type1, IHhas_type2. rewrite (eqb_ty_refl T11)...
+
+  1 - 2 : auto.
+
+  rewrite IHhas_type1, IHhas_type2, IHhas_type3, (eqb_ty_refl T)...
+Qed.
+
+(* Leaving Exercises *)
